ugly sums, but finished sums

code/theories/Ast.sig
@@ -2,6 +2,7 @@ base : Type
 bool : Type
 type : Type
 term(tVar) : Type
+elim : Type
 
 TBase : base -> type
 
@@ -15,3 +16,15 @@ tProj : bool -> term -> term
 TFun : type -> type -> type
 tLam : (bind term in term) -> term
 tApp : term -> term -> term
+
+TEmp : type
+tAbort : term -> term
+
+TSum : type -> type -> type
+tIn : bool -> term -> term
+tIf : term -> (bind term in term) -> (bind term in term) -> term
+
+eProj : bool -> elim
+eApp : term -> elim
+eAbort : elim
+eIf : (bind term in term) -> (bind term in term) -> elim
