code/theories/Ast.v
@@ -11,7 +11,10 @@ Inductive term : Type :=
   | tPair : term -> term -> term
   | tProj : bool -> term -> term
   | tLam : term -> term
-  | tApp : term -> term -> term.
+  | tApp : term -> term -> term
+  | tAbort : term -> term
+  | tIn : bool -> term -> term
+  | tIf : term -> term -> term -> term.
 
 Lemma congr_tStar : tStar = tStar.
 Proof.
@@ -44,6 +47,29 @@ exact (eq_trans (eq_trans eq_refl (ap (fun x => tApp x s1) H0))
          (ap (fun x => tApp t0 x) H1)).
 Qed.
 
+Lemma congr_tAbort {s0 : term} {t0 : term} (H0 : s0 = t0) :
+  tAbort s0 = tAbort t0.
+Proof.
+exact (eq_trans eq_refl (ap (fun x => tAbort x) H0)).
+Qed.
+
+Lemma congr_tIn {s0 : bool} {s1 : term} {t0 : bool} {t1 : term}
+  (H0 : s0 = t0) (H1 : s1 = t1) : tIn s0 s1 = tIn t0 t1.
+Proof.
+exact (eq_trans (eq_trans eq_refl (ap (fun x => tIn x s1) H0))
+         (ap (fun x => tIn t0 x) H1)).
+Qed.
+
+Lemma congr_tIf {s0 : term} {s1 : term} {s2 : term} {t0 : term} {t1 : term}
+  {t2 : term} (H0 : s0 = t0) (H1 : s1 = t1) (H2 : s2 = t2) :
+  tIf s0 s1 s2 = tIf t0 t1 t2.
+Proof.
+exact (eq_trans
+         (eq_trans (eq_trans eq_refl (ap (fun x => tIf x s1 s2) H0))
+            (ap (fun x => tIf t0 x s2) H1))
+         (ap (fun x => tIf t0 t1 x) H2)).
+Qed.
+
 Lemma upRen_term_term (xi : nat -> nat) : nat -> nat.
 Proof.
 exact (up_ren xi).
@@ -57,6 +83,11 @@ Fixpoint ren_term (xi_term : nat -> nat) (s : term) {struct s} : term :=
   | tProj s0 s1 => tProj s0 (ren_term xi_term s1)
   | tLam s0 => tLam (ren_term (upRen_term_term xi_term) s0)
   | tApp s0 s1 => tApp (ren_term xi_term s0) (ren_term xi_term s1)
+  | tAbort s0 => tAbort (ren_term xi_term s0)
+  | tIn s0 s1 => tIn s0 (ren_term xi_term s1)
+  | tIf s0 s1 s2 =>
+      tIf (ren_term xi_term s0) (ren_term (upRen_term_term xi_term) s1)
+        (ren_term (upRen_term_term xi_term) s2)
   end.
 
 Lemma up_term_term (sigma : nat -> term) : nat -> term.
@@ -74,6 +105,12 @@ term :=
   | tProj s0 s1 => tProj s0 (subst_term sigma_term s1)
   | tLam s0 => tLam (subst_term (up_term_term sigma_term) s0)
   | tApp s0 s1 => tApp (subst_term sigma_term s0) (subst_term sigma_term s1)
+  | tAbort s0 => tAbort (subst_term sigma_term s0)
+  | tIn s0 s1 => tIn s0 (subst_term sigma_term s1)
+  | tIf s0 s1 s2 =>
+      tIf (subst_term sigma_term s0)
+        (subst_term (up_term_term sigma_term) s1)
+        (subst_term (up_term_term sigma_term) s2)
   end.
 
 Lemma upId_term_term (sigma : nat -> term) (Eq : forall x, sigma x = tVar x)
@@ -103,6 +140,12 @@ subst_term sigma_term s = s :=
   | tApp s0 s1 =>
       congr_tApp (idSubst_term sigma_term Eq_term s0)
         (idSubst_term sigma_term Eq_term s1)
+  | tAbort s0 => congr_tAbort (idSubst_term sigma_term Eq_term s0)
+  | tIn s0 s1 => congr_tIn (eq_refl s0) (idSubst_term sigma_term Eq_term s1)
+  | tIf s0 s1 s2 =>
+      congr_tIf (idSubst_term sigma_term Eq_term s0)
+        (idSubst_term (up_term_term sigma_term) (upId_term_term _ Eq_term) s1)
+        (idSubst_term (up_term_term sigma_term) (upId_term_term _ Eq_term) s2)
   end.
 
 Lemma upExtRen_term_term (xi : nat -> nat) (zeta : nat -> nat)
@@ -133,6 +176,15 @@ ren_term xi_term s = ren_term zeta_term s :=
   | tApp s0 s1 =>
       congr_tApp (extRen_term xi_term zeta_term Eq_term s0)
         (extRen_term xi_term zeta_term Eq_term s1)
+  | tAbort s0 => congr_tAbort (extRen_term xi_term zeta_term Eq_term s0)
+  | tIn s0 s1 =>
+      congr_tIn (eq_refl s0) (extRen_term xi_term zeta_term Eq_term s1)
+  | tIf s0 s1 s2 =>
+      congr_tIf (extRen_term xi_term zeta_term Eq_term s0)
+        (extRen_term (upRen_term_term xi_term) (upRen_term_term zeta_term)
+           (upExtRen_term_term _ _ Eq_term) s1)
+        (extRen_term (upRen_term_term xi_term) (upRen_term_term zeta_term)
+           (upExtRen_term_term _ _ Eq_term) s2)
   end.
 
 Lemma upExt_term_term (sigma : nat -> term) (tau : nat -> term)
@@ -164,6 +216,15 @@ subst_term sigma_term s = subst_term tau_term s :=
   | tApp s0 s1 =>
       congr_tApp (ext_term sigma_term tau_term Eq_term s0)
         (ext_term sigma_term tau_term Eq_term s1)
+  | tAbort s0 => congr_tAbort (ext_term sigma_term tau_term Eq_term s0)
+  | tIn s0 s1 =>
+      congr_tIn (eq_refl s0) (ext_term sigma_term tau_term Eq_term s1)
+  | tIf s0 s1 s2 =>
+      congr_tIf (ext_term sigma_term tau_term Eq_term s0)
+        (ext_term (up_term_term sigma_term) (up_term_term tau_term)
+           (upExt_term_term _ _ Eq_term) s1)
+        (ext_term (up_term_term sigma_term) (up_term_term tau_term)
+           (upExt_term_term _ _ Eq_term) s2)
   end.
 
 Lemma up_ren_ren_term_term (xi : nat -> nat) (zeta : nat -> nat)
@@ -196,6 +257,19 @@ Fixpoint compRenRen_term (xi_term : nat -> nat) (zeta_term : nat -> nat)
   | tApp s0 s1 =>
       congr_tApp (compRenRen_term xi_term zeta_term rho_term Eq_term s0)
         (compRenRen_term xi_term zeta_term rho_term Eq_term s1)
+  | tAbort s0 =>
+      congr_tAbort (compRenRen_term xi_term zeta_term rho_term Eq_term s0)
+  | tIn s0 s1 =>
+      congr_tIn (eq_refl s0)
+        (compRenRen_term xi_term zeta_term rho_term Eq_term s1)
+  | tIf s0 s1 s2 =>
+      congr_tIf (compRenRen_term xi_term zeta_term rho_term Eq_term s0)
+        (compRenRen_term (upRen_term_term xi_term)
+           (upRen_term_term zeta_term) (upRen_term_term rho_term)
+           (up_ren_ren _ _ _ Eq_term) s1)
+        (compRenRen_term (upRen_term_term xi_term)
+           (upRen_term_term zeta_term) (upRen_term_term rho_term)
+           (up_ren_ren _ _ _ Eq_term) s2)
   end.
 
 Lemma up_ren_subst_term_term (xi : nat -> nat) (tau : nat -> term)
@@ -232,6 +306,19 @@ subst_term tau_term (ren_term xi_term s) = subst_term theta_term s :=
   | tApp s0 s1 =>
       congr_tApp (compRenSubst_term xi_term tau_term theta_term Eq_term s0)
         (compRenSubst_term xi_term tau_term theta_term Eq_term s1)
+  | tAbort s0 =>
+      congr_tAbort (compRenSubst_term xi_term tau_term theta_term Eq_term s0)
+  | tIn s0 s1 =>
+      congr_tIn (eq_refl s0)
+        (compRenSubst_term xi_term tau_term theta_term Eq_term s1)
+  | tIf s0 s1 s2 =>
+      congr_tIf (compRenSubst_term xi_term tau_term theta_term Eq_term s0)
+        (compRenSubst_term (upRen_term_term xi_term) (up_term_term tau_term)
+           (up_term_term theta_term) (up_ren_subst_term_term _ _ _ Eq_term)
+           s1)
+        (compRenSubst_term (upRen_term_term xi_term) (up_term_term tau_term)
+           (up_term_term theta_term) (up_ren_subst_term_term _ _ _ Eq_term)
+           s2)
   end.
 
 Lemma up_subst_ren_term_term (sigma : nat -> term) (zeta_term : nat -> nat)
@@ -280,6 +367,21 @@ ren_term zeta_term (subst_term sigma_term s) = subst_term theta_term s :=
       congr_tApp
         (compSubstRen_term sigma_term zeta_term theta_term Eq_term s0)
         (compSubstRen_term sigma_term zeta_term theta_term Eq_term s1)
+  | tAbort s0 =>
+      congr_tAbort
+        (compSubstRen_term sigma_term zeta_term theta_term Eq_term s0)
+  | tIn s0 s1 =>
+      congr_tIn (eq_refl s0)
+        (compSubstRen_term sigma_term zeta_term theta_term Eq_term s1)
+  | tIf s0 s1 s2 =>
+      congr_tIf
+        (compSubstRen_term sigma_term zeta_term theta_term Eq_term s0)
+        (compSubstRen_term (up_term_term sigma_term)
+           (upRen_term_term zeta_term) (up_term_term theta_term)
+           (up_subst_ren_term_term _ _ _ Eq_term) s1)
+        (compSubstRen_term (up_term_term sigma_term)
+           (upRen_term_term zeta_term) (up_term_term theta_term)
+           (up_subst_ren_term_term _ _ _ Eq_term) s2)
   end.
 
 Lemma up_subst_subst_term_term (sigma : nat -> term) (tau_term : nat -> term)
@@ -331,6 +433,21 @@ subst_term tau_term (subst_term sigma_term s) = subst_term theta_term s :=
       congr_tApp
         (compSubstSubst_term sigma_term tau_term theta_term Eq_term s0)
         (compSubstSubst_term sigma_term tau_term theta_term Eq_term s1)
+  | tAbort s0 =>
+      congr_tAbort
+        (compSubstSubst_term sigma_term tau_term theta_term Eq_term s0)
+  | tIn s0 s1 =>
+      congr_tIn (eq_refl s0)
+        (compSubstSubst_term sigma_term tau_term theta_term Eq_term s1)
+  | tIf s0 s1 s2 =>
+      congr_tIf
+        (compSubstSubst_term sigma_term tau_term theta_term Eq_term s0)
+        (compSubstSubst_term (up_term_term sigma_term)
+           (up_term_term tau_term) (up_term_term theta_term)
+           (up_subst_subst_term_term _ _ _ Eq_term) s1)
+        (compSubstSubst_term (up_term_term sigma_term)
+           (up_term_term tau_term) (up_term_term theta_term)
+           (up_subst_subst_term_term _ _ _ Eq_term) s2)
   end.
 
 Lemma renRen_term (xi_term : nat -> nat) (zeta_term : nat -> nat) (s : term)
@@ -430,6 +547,15 @@ Fixpoint rinst_inst_term (xi_term : nat -> nat) (sigma_term : nat -> term)
   | tApp s0 s1 =>
       congr_tApp (rinst_inst_term xi_term sigma_term Eq_term s0)
         (rinst_inst_term xi_term sigma_term Eq_term s1)
+  | tAbort s0 => congr_tAbort (rinst_inst_term xi_term sigma_term Eq_term s0)
+  | tIn s0 s1 =>
+      congr_tIn (eq_refl s0) (rinst_inst_term xi_term sigma_term Eq_term s1)
+  | tIf s0 s1 s2 =>
+      congr_tIf (rinst_inst_term xi_term sigma_term Eq_term s0)
+        (rinst_inst_term (upRen_term_term xi_term) (up_term_term sigma_term)
+           (rinstInst_up_term_term _ _ Eq_term) s1)
+        (rinst_inst_term (upRen_term_term xi_term) (up_term_term sigma_term)
+           (rinstInst_up_term_term _ _ Eq_term) s2)
   end.
 
 Lemma rinstInst'_term (xi_term : nat -> nat) (s : term) :
@@ -491,11 +617,130 @@ Proof.
 exact (fun x => eq_refl).
 Qed.
 
+Inductive elim : Type :=
+  | eProj : bool -> elim
+  | eApp : term -> elim
+  | eAbort : elim
+  | eIf : term -> term -> elim.
+
+Lemma congr_eProj {s0 : bool} {t0 : bool} (H0 : s0 = t0) :
+  eProj s0 = eProj t0.
+Proof.
+exact (eq_trans eq_refl (ap (fun x => eProj x) H0)).
+Qed.
+
+Lemma congr_eApp {s0 : term} {t0 : term} (H0 : s0 = t0) : eApp s0 = eApp t0.
+Proof.
+exact (eq_trans eq_refl (ap (fun x => eApp x) H0)).
+Qed.
+
+Lemma congr_eAbort : eAbort = eAbort.
+Proof.
+exact (eq_refl).
+Qed.
+
+Lemma congr_eIf {s0 : term} {s1 : term} {t0 : term} {t1 : term}
+  (H0 : s0 = t0) (H1 : s1 = t1) : eIf s0 s1 = eIf t0 t1.
+Proof.
+exact (eq_trans (eq_trans eq_refl (ap (fun x => eIf x s1) H0))
+         (ap (fun x => eIf t0 x) H1)).
+Qed.
+
+Definition subst_elim (sigma_term : nat -> term) (s : elim) : elim :=
+  match s with
+  | eProj s0 => eProj s0
+  | eApp s0 => eApp (subst_term sigma_term s0)
+  | eAbort => eAbort
+  | eIf s0 s1 =>
+      eIf (subst_term (up_term_term sigma_term) s0)
+        (subst_term (up_term_term sigma_term) s1)
+  end.
+
+Definition idSubst_elim (sigma_term : nat -> term)
+  (Eq_term : forall x, sigma_term x = tVar x) (s : elim) :
+  subst_elim sigma_term s = s :=
+  match s with
+  | eProj s0 => congr_eProj (eq_refl s0)
+  | eApp s0 => congr_eApp (idSubst_term sigma_term Eq_term s0)
+  | eAbort => congr_eAbort
+  | eIf s0 s1 =>
+      congr_eIf
+        (idSubst_term (up_term_term sigma_term) (upId_term_term _ Eq_term) s0)
+        (idSubst_term (up_term_term sigma_term) (upId_term_term _ Eq_term) s1)
+  end.
+
+Definition ext_elim (sigma_term : nat -> term) (tau_term : nat -> term)
+  (Eq_term : forall x, sigma_term x = tau_term x) (s : elim) :
+  subst_elim sigma_term s = subst_elim tau_term s :=
+  match s with
+  | eProj s0 => congr_eProj (eq_refl s0)
+  | eApp s0 => congr_eApp (ext_term sigma_term tau_term Eq_term s0)
+  | eAbort => congr_eAbort
+  | eIf s0 s1 =>
+      congr_eIf
+        (ext_term (up_term_term sigma_term) (up_term_term tau_term)
+           (upExt_term_term _ _ Eq_term) s0)
+        (ext_term (up_term_term sigma_term) (up_term_term tau_term)
+           (upExt_term_term _ _ Eq_term) s1)
+  end.
+
+Definition compSubstSubst_elim (sigma_term : nat -> term)
+  (tau_term : nat -> term) (theta_term : nat -> term)
+  (Eq_term : forall x,
+             funcomp (subst_term tau_term) sigma_term x = theta_term x)
+  (s : elim) :
+  subst_elim tau_term (subst_elim sigma_term s) = subst_elim theta_term s :=
+  match s with
+  | eProj s0 => congr_eProj (eq_refl s0)
+  | eApp s0 =>
+      congr_eApp
+        (compSubstSubst_term sigma_term tau_term theta_term Eq_term s0)
+  | eAbort => congr_eAbort
+  | eIf s0 s1 =>
+      congr_eIf
+        (compSubstSubst_term (up_term_term sigma_term)
+           (up_term_term tau_term) (up_term_term theta_term)
+           (up_subst_subst_term_term _ _ _ Eq_term) s0)
+        (compSubstSubst_term (up_term_term sigma_term)
+           (up_term_term tau_term) (up_term_term theta_term)
+           (up_subst_subst_term_term _ _ _ Eq_term) s1)
+  end.
+
+Lemma substSubst_elim (sigma_term : nat -> term) (tau_term : nat -> term)
+  (s : elim) :
+  subst_elim tau_term (subst_elim sigma_term s) =
+  subst_elim (funcomp (subst_term tau_term) sigma_term) s.
+Proof.
+exact (compSubstSubst_elim sigma_term tau_term _ (fun n => eq_refl) s).
+Qed.
+
+Lemma substSubst_elim_pointwise (sigma_term : nat -> term)
+  (tau_term : nat -> term) :
+  pointwise_relation _ eq
+    (funcomp (subst_elim tau_term) (subst_elim sigma_term))
+    (subst_elim (funcomp (subst_term tau_term) sigma_term)).
+Proof.
+exact (fun s =>
+       compSubstSubst_elim sigma_term tau_term _ (fun n => eq_refl) s).
+Qed.
+
+Lemma instId'_elim (s : elim) : subst_elim (tVar) s = s.
+Proof.
+exact (idSubst_elim (tVar) (fun n => eq_refl) s).
+Qed.
+
+Lemma instId'_elim_pointwise : pointwise_relation _ eq (subst_elim (tVar)) id.
+Proof.
+exact (fun s => idSubst_elim (tVar) (fun n => eq_refl) s).
+Qed.
+
 Inductive type : Type :=
   | TBase : base -> type
   | TUnit : type
   | TProd : type -> type -> type
-  | TFun : type -> type -> type.
+  | TFun : type -> type -> type
+  | TEmp : type
+  | TSum : type -> type -> type.
 
 Lemma congr_TBase {s0 : base} {t0 : base} (H0 : s0 = t0) :
   TBase s0 = TBase t0.
@@ -522,8 +767,25 @@ exact (eq_trans (eq_trans eq_refl (ap (fun x => TFun x s1) H0))
          (ap (fun x => TFun t0 x) H1)).
 Qed.
 
+Lemma congr_TEmp : TEmp = TEmp.
+Proof.
+exact (eq_refl).
+Qed.
+
+Lemma congr_TSum {s0 : type} {s1 : type} {t0 : type} {t1 : type}
+  (H0 : s0 = t0) (H1 : s1 = t1) : TSum s0 s1 = TSum t0 t1.
+Proof.
+exact (eq_trans (eq_trans eq_refl (ap (fun x => TSum x s1) H0))
+         (ap (fun x => TSum t0 x) H1)).
+Qed.
+
+Class Up_elim X Y :=
+    up_elim : X -> Y.
+
 Class Up_term X Y :=
     up_term : X -> Y.
+
+#[global] Instance Subst_elim : (Subst1 _ _ _) := @subst_elim.
 
 #[global] Instance Subst_term : (Subst1 _ _ _) := @subst_term.
 
@@ -533,6 +795,11 @@ Class Up_term X Y :=
 
 #[global]
 Instance VarInstance_term : (Var _ _) := @tVar.
+
+Notation "s [ sigma_term ]" := (subst_elim sigma_term s)
+( at level 7, left associativity, only printing)  : subst_scope.
+
+Notation "↑__elim" := up_elim (only printing)  : subst_scope.
 
 Notation "s [ sigma_term ]" := (subst_term sigma_term s)
 ( at level 7, left associativity, only printing)  : subst_scope.
@@ -551,6 +818,24 @@ Notation "x '__term'" := (@ids _ _ VarInstance_term x)
 
 Notation "x '__term'" := (tVar x) ( at level 5, format "x __term")  :
 subst_scope.
+
+#[global]
+Instance subst_elim_morphism :
+ (Proper (respectful (pointwise_relation _ eq) (respectful eq eq))
+    (@subst_elim)).
+Proof.
+exact (fun f_term g_term Eq_term s t Eq_st =>
+       eq_ind s (fun t' => subst_elim f_term s = subst_elim g_term t')
+         (ext_elim f_term g_term Eq_term s) t Eq_st).
+Qed.
+
+#[global]
+Instance subst_elim_morphism2 :
+ (Proper (respectful (pointwise_relation _ eq) (pointwise_relation _ eq))
+    (@subst_elim)).
+Proof.
+exact (fun f_term g_term Eq_term s => ext_elim f_term g_term Eq_term s).
+Qed.
 
 #[global]
 Instance subst_term_morphism :
@@ -591,17 +876,20 @@ Qed.
 Ltac auto_unfold := repeat
                      unfold VarInstance_term, Var, ids, Ren_term, Ren1, ren1,
                       Up_term_term, Up_term, up_term, Subst_term, Subst1,
-                      subst1.
+                      subst1, Subst_elim, Subst1, subst1.
 
 Tactic Notation "auto_unfold" "in" "*" := repeat
                                            unfold VarInstance_term, Var, ids,
                                             Ren_term, Ren1, ren1,
                                             Up_term_term, Up_term, up_term,
-                                            Subst_term, Subst1, subst1 
+                                            Subst_term, Subst1, subst1,
+                                            Subst_elim, Subst1, subst1 
                                             in *.
 
 Ltac asimpl' := repeat (first
-                 [ progress setoid_rewrite substSubst_term_pointwise
+                 [ progress setoid_rewrite substSubst_elim_pointwise
+                 | progress setoid_rewrite substSubst_elim
+                 | progress setoid_rewrite substSubst_term_pointwise
                  | progress setoid_rewrite substSubst_term
                  | progress setoid_rewrite substRen_term_pointwise
                  | progress setoid_rewrite substRen_term
@@ -609,6 +897,8 @@ Ltac asimpl' := repeat (first
                  | progress setoid_rewrite renSubst_term
                  | progress setoid_rewrite renRen'_term_pointwise
                  | progress setoid_rewrite renRen_term
+                 | progress setoid_rewrite instId'_elim_pointwise
+                 | progress setoid_rewrite instId'_elim
                  | progress setoid_rewrite varLRen'_term_pointwise
                  | progress setoid_rewrite varLRen'_term
                  | progress setoid_rewrite varL'_term_pointwise
@@ -618,14 +908,14 @@ Ltac asimpl' := repeat (first
                  | progress setoid_rewrite instId'_term_pointwise
                  | progress setoid_rewrite instId'_term
                  | progress unfold up_term_term, upRen_term_term, up_ren
-                 | progress cbn[subst_term ren_term]
+                 | progress cbn[subst_elim subst_term ren_term]
                  | progress fsimpl ]).
 
 Ltac asimpl := check_no_evars;
                 repeat
                  unfold VarInstance_term, Var, ids, Ren_term, Ren1, ren1,
-                  Up_term_term, Up_term, up_term, Subst_term, Subst1, subst1
-                  in *;
+                  Up_term_term, Up_term, up_term, Subst_term, Subst1, subst1,
+                  Subst_elim, Subst1, subst1 in *;
                 asimpl'; minimize.
 
 Tactic Notation "asimpl" "in" hyp(J) := revert J; asimpl; intros J.
@@ -644,6 +934,8 @@ End Core.
 Module Extra.
 
 Import Core.
+
+#[global] Hint Opaque subst_elim: rewrite.
 
 #[global] Hint Opaque subst_term: rewrite.
 
