code/theories/Syntax.v
@@ -1,5 +1,6 @@
 From smpl Require Import Smpl.
 From Stdlib Require Import ssrbool List.
+From Stdlib Require Import Setoid Morphisms Relation_Definitions RelationClasses.
 From Interpolation Require Export BasicAst core unscoped Ast Context.
 From Interpolation Require Import Utils.
 
@@ -31,12 +32,22 @@ Notation "s '..'" := (scons s ids) (at level 1, format "s ..") : asubst_scope.
 
 Notation "↑" := (shift) : asubst_scope.
 
-Notation "⇑ σ" := (up_term_term σ) (at level 1) : asubst_scope.
+Notation "⇑ σ" := (up_term σ) (at level 1) : asubst_scope.
+
+#[global] Instance up_term_ren : Up_term _ _ := up_ren.
+
+Arguments up_term_ren _/.
 
 #[global] Open Scope asubst_scope.
 
 Notation "'tFst'" := (tProj true).
 Notation "'tSnd'" := (tProj false).
+Notation "'eFst'" := (eProj true).
+Notation "'eSnd'" := (eProj false).
+Notation "'tLeft'" := (tIn false).
+Notation "'tRight'" := (tIn true).
+
+#[global] Instance Ren_elim : (Ren1 (nat -> nat) elim elim) := fun ρ e => @subst_elim (ρ >> tVar) e.
 
 #[global] Instance Ren1_subst {Y Z : Type} `{Ren1 (nat -> nat) Y Z} :
   (Ren1 (nat -> nat) (nat -> Y) (nat -> Z)) :=
@@ -44,14 +55,18 @@ Notation "'tSnd'" := (tProj false).
 
 Ltac fold_autosubst :=
     fold ren_term ;
-    fold subst_term.
+    fold subst_term ;
+    fold subst_elim.
 
 Smpl Add fold_autosubst : refold.
 
 Ltac change_autosubst :=
     change ren_term with (@ren1 _ _ _ Ren_term) in * ;
     change subst_term with (@subst1 _ _ _ Subst_term) in *;
-    change (fun i => (?σ i)⟨?ρ⟩) with (@ren1 _ _ _ Ren1_subst ρ σ) in *.
+    change (fun i => (?σ i)⟨?ρ⟩) with (@ren1 _ _ _ Ren1_subst ρ σ) in * ;
+    change up_ren with (@up_term _ _ up_term_ren) in * ;
+    change upRen_term_term with (@up_term _ _ up_term_ren) in * ;
+    change up_term_term with (@up_term _ _ Up_term_term) in *.
 
 Smpl Add 50 change_autosubst : refold.
 
@@ -61,3 +76,74 @@ Arguments Ren_term _ _ /.
 Arguments Ren1_subst {_ _ _} _ _/.
 Arguments ids {_ _} {_} _/.
 Arguments VarInstance_term _/.
+
+(** ** Lemmas *)
+
+Lemma subst1_ren (t u : term) (ρ : ren) : t[u..]⟨ρ⟩ = t⟨⇑ ρ⟩[u⟨ρ⟩..].
+Proof.
+  now substify ; asimpl.
+Qed.
+
+Lemma subst1_subst (t u : term) (σ : subst) : t[u..][σ] = t[⇑ σ][u[σ]..].
+Proof.
+  now asimpl.
+Qed.
+
+Lemma elim_ren e ρ : e⟨ρ⟩ = e[ρ >> tVar].
+Proof.
+  substify ; refold.
+  reflexivity.
+Qed.
+
+Definition tip (f : term -> term) : subst :=  (f (tVar 0)).: (↑ >> ids).
+
+Lemma tip_subst (f : term -> term) (t u : term) :
+  (forall σ x, (f x) [σ] = f (x[σ])) ->
+  u[tip f][t ..] = u[(f t)..].
+Proof.
+  intros Hf.
+  rewrite substSubst_term ; refold.
+  apply ext_term.
+  intros x.
+  unfold tip.
+  asimpl ; cbn.
+  destruct x ; cbn ; [|easy].
+  rewrite Hf ; asimpl.
+  reflexivity.
+Qed.
+
+Lemma tip_shift (f : term -> term) ρ (t : term) :
+  (forall σ x, (f x) [σ] = f (x[σ])) ->
+  t[tip f]⟨⇑ ρ⟩ = t⟨⇑ ρ⟩[tip f].
+Proof.
+  intros Hf.
+  unfold tip.
+  substify ; asimpl.
+  rewrite Hf ; asimpl.
+  reflexivity.
+Qed.
+
+Definition swap_var : ren :=
+  1 .: (0 .: (↑ >> ↑)).
+
+Lemma swap_shift2 ρ (t : term) :
+  t⟨swap_var⟩⟨⇑ ⇑ ρ⟩ = t⟨⇑ ⇑ ρ⟩⟨swap_var⟩.
+Proof.
+  unfold swap_var.
+  asimpl ; reflexivity.
+Qed.
+
+Lemma swap_shift1 (t u : term) :
+  t⟨swap_var⟩[⇑ (u..)] = t[u⟨↑⟩..].
+Proof.
+  unfold swap_var.
+  substify ; asimpl ; renamify ; refold.
+  now rewrite scons_eta'.
+Qed.
+
+Lemma swap_subst1 (t u : term) :
+  t⟨swap_var⟩[(u⟨↑⟩ ..)] = t[⇑ (u..)].
+Proof.
+  unfold swap_var.
+  substify ; asimpl ; substify ; reflexivity.
+Qed.
