code/theories/Bidir.v
@@ -1,4 +1,4 @@
-From Interpolation Require Import Utils Syntax Typing.
+From Interpolation Require Import Utils Syntax Notations Typing.
 From Stdlib Require Import Relations Arith Lia Bool List.
 
 Reserved Notation "Γ '|-' t ▹ T"
@@ -8,11 +8,11 @@ Reserved Notation "Γ '|-' t ◃ T"
 
 Unset Elimination Schemes.
 
-Inductive check : context -> type -> term -> Prop :=
+Inductive normal : context -> type -> term -> Prop :=
 | C_Star Γ : (Γ |- tStar ◃ TUnit)
 
 | C_Abs Γ (A B : type) t :
-  (Γ ,,, A |- t ◃ B) ->
+  (Γ ,, A |- t ◃ B) ->
   Γ |- tLam t ◃ TFun A B
 
 | C_Pair Γ A B a b :
@@ -20,12 +20,30 @@ Inductive check : context -> type -> term -> Prop :=
   (Γ |- b ◃ B) ->
   (Γ |- tPair a b ◃ TProd A B)
 
+| C_Left Γ A B a :
+  (Γ |- a ◃ A) ->
+  (Γ |- tLeft a ◃ TSum A B)
+
+| C_Right Γ A B b :
+  (Γ |- b ◃ B) ->
+  (Γ |- tRight b ◃ TSum A B)
+
+| C_Abort Γ A t :
+  (Γ |- t ◃ TEmp) ->
+  (Γ |- tAbort t ◃ A)
+
+| C_If Γ A B T s bl br :
+  (Γ |- s ▹ TSum A B) ->
+  (Γ,,A |- bl ◃ T) ->
+  (Γ,,B |- br ◃ T) ->
+  (Γ |- tIf s bl br ◃ T)
+
 | C_inf Γ A A' t :
   (Γ |- t ▹ A') ->
   A' = A ->
   (Γ |- t ◃ A)
 
-with infer : context -> type -> term -> Prop :=
+with neutral : context -> type -> term -> Prop :=
 | I_Var Γ n T :
   in_context n Γ T ->
   Γ |- tVar n ▹ T
@@ -39,16 +57,16 @@ with infer : context -> type -> term -> Prop :=
   (Γ |- t ▹ TProd A B) ->
   (Γ |- tProj b t ▹ (if b then A else B))
 
-where "Γ '|-' t ▹ T" := (infer Γ T t) (Γ in scope context_scope)
-and "Γ '|-' t ◃ T" := (check Γ T t) (Γ in scope context_scope).
+where "Γ '|-' t ▹ T" := (neutral Γ T t) (Γ in scope context_scope)
+and "Γ '|-' t ◃ T" := (normal Γ T t) (Γ in scope context_scope).
 
-Hint Constructors check infer : core.
+Hint Constructors neutral normal : core.
 
 Scheme 
-Minimality for check Sort Prop with
-Minimality for infer Sort Prop.
+Minimality for normal Sort Prop with
+Minimality for neutral Sort Prop.
 
-Combined Scheme bidir_ind from check_ind, infer_ind.
+Combined Scheme bidir_ind from normal_ind, neutral_ind.
 
 Definition bidir_concl :=
 ltac:(
@@ -56,4 +74,15 @@ let t := type of bidir_ind in
 let t' := remove_steps t in
 exact t').
 
-Arguments bidir_concl Pcheck Pinf : rename.
+Arguments bidir_concl Pnf Pne : rename.
+
+
+Theorem bidir_typing : bidir_concl (fun Γ T t => (Γ |- t :: T)) (fun Γ T t => (Γ |- t :: T)).
+Proof.
+  apply bidir_ind.
+  all: try solve [now econstructor].
+  - intros ; now subst.
+  - intros.
+    destruct b.
+    all: now econstructor.
+Qed.
