code/theories/Context.v
@@ -15,15 +15,15 @@ Fixpoint nth_error {A} (l : list A) (n : nat) : option A :=
 Definition context := list type.
 
 Notation "'ε'" := (@nil type).
-Notation "Γ ,,, T" := (@cons type T Γ) (at level 50).
+Notation "Γ ,, T" := (@cons type T Γ) (at level 50).
 (* 
 Notation "'ε'" := (nil :> context) (only parsing).
-Notation "Γ ,,, T" := (cons T Γ :> context) (at level 50, only parsing). *)
+Notation "Γ ,, T" := (cons T Γ :> context) (at level 50, only parsing). *)
 
 Definition in_context (n : nat) (Γ : context) (T : type) : Prop :=
   nth_error Γ n = Some T.
 
-Lemma in_zero Γ T : in_context 0 (Γ,,,T) T.
+Lemma in_zero Γ T : in_context 0 (Γ,,T) T.
 Proof. reflexivity. Qed.
 
 Hint Resolve in_zero : core.
