code/theories/Elim.v
@@ -1,0 +1,23 @@
+From Interpolation Require Import Utils Syntax Notations.
+From Stdlib Require Import Setoid Morphisms Relation_Definitions RelationClasses.
+From Stdlib Require Import Relations Arith Lia Bool List.
+
+Import ListNotations.
+
+Definition zip (e : elim) (t : term) : term :=
+  match e with
+  | eProj b => tProj b t
+  | eApp u => tApp t u
+  | eAbort => tAbort t
+  | eIf bl br => tIf t bl br
+  end.
+
+Lemma zip_subst e t (σ : subst) : (zip e t)[σ] = zip (e[σ]) (t[σ]).
+Proof.
+  destruct e ; reflexivity.
+Qed.
+
+Lemma zip_ren e t (ρ : ren) : (zip e t)⟨ρ⟩ = zip (e⟨ρ⟩) (t⟨ρ⟩).
+Proof.
+  substify ; apply zip_subst.
+Qed.
